make c,v short but symbols

chapter05/exercises/exercise01.dfy
@@ -19,36 +19,36 @@ module MapSpec {
 
   datatype Variables = Variables(m:map<Key, Value>)
 
-  predicate Init(v: Variables)
+  predicate Init(v_: Variables)
   {
-    v.m == map[]
+    v_.m == map[]
   }
 
-  predicate InsertOp(v:Variables, v':Variables, k:Key, value:Value)
+  predicate InsertOp(v_:Variables, v_':Variables, k:Key, value:Value)
   {
-    v'.m == v.m[k := value]
+    v_'.m == v_.m[k := value]
   }
 
-  predicate QueryOp(v:Variables, v':Variables, k:Key, output:Value)
+  predicate QueryOp(v_:Variables, v_':Variables, k:Key, output:Value)
   {
-    && (output == if k in v.m then v.m[k] else DefaultValue())
-    && v' == v  // no change to map state
+    && (output == if k in v_.m then v_.m[k] else DefaultValue())
+    && v_' == v_  // no change to map state
   }
 
   datatype Step =
     | InsertOpStep(k:Key, value:Value)
     | QueryOpStep(k:Key, output:Value)
 
-  predicate NextStep(v: Variables, v': Variables, step:Step)
+  predicate NextStep(v_: Variables, v_': Variables, step:Step)
   {
     match step
-      case InsertOpStep(k, value) => InsertOp(v, v', k, value)
-      case QueryOpStep(k, output) => QueryOp(v, v', k, output)
+      case InsertOpStep(k, value) => InsertOp(v_, v_', k, value)
+      case QueryOpStep(k, output) => QueryOp(v_, v_', k, output)
   }
 
-  predicate Next(v: Variables, v': Variables)
+  predicate Next(v_: Variables, v_': Variables)
   {
-    exists step :: NextStep(v, v', step)
+    exists step :: NextStep(v_, v_', step)
   }
 }
 
@@ -63,32 +63,32 @@ module Host {
     // if a key is absent, only the manager can spring it
     // into existence.
 
-  predicate Init(c: Constants, v: Variables, i: nat)
+  predicate Init(c_: Constants, v_: Variables, i: nat)
   {
-    && c.manager == (i==0)
-    && v.m == map[]
+    && c_.manager == (i==0)
+    && v_.m == map[]
   }
 
-  predicate Insert(c: Constants, v: Variables, v': Variables, k: Key, value: Value)
+  predicate Insert(c_: Constants, v_: Variables, v_': Variables, k: Key, value: Value)
   {
-    && k in v.m // this host needs to be authoritative on this key
-    && v'.m == v.m[k := value]
+    && k in v_.m // this host needs to be authoritative on this key
+    && v_'.m == v_.m[k := value]
   }
 
-  predicate Query(c: Constants, v: Variables, v': Variables, k: Key, output: Value)
+  predicate Query(c_: Constants, v_: Variables, v_': Variables, k: Key, output: Value)
   {
-    && k in v.m
-    && output == v.m[k]
-    && v' == v  // UNCHANGED
+    && k in v_.m
+    && output == v_.m[k]
+    && v_' == v_  // UNCHANGED
   }
 
   // This is how we allow other hosts to serve queries for missing
   // keys: we insert an explicit value to get the key into our map.
-  predicate FillDefault(c: Constants, v: Variables, v': Variables, k: Key)
+  predicate FillDefault(c_: Constants, v_: Variables, v_': Variables, k: Key)
   {
-    && c.manager  // only manager is authoritative on missing keys
-    && k !in v.m
-    && v'.m == v.m[k := DefaultValue()]
+    && c_.manager  // only manager is authoritative on missing keys
+    && k !in v_.m
+    && v_'.m == v_.m[k := DefaultValue()]
   }
 
   datatype Step =
@@ -96,17 +96,17 @@ module Host {
     | QueryStep(k: Key, output: Value)
     | FillDefaultStep(k: Key)
 
-  predicate LocalOpStep(c: Constants, v: Variables, v': Variables, step: Step)
+  predicate LocalOpStep(c_: Constants, v_: Variables, v_': Variables, step: Step)
   {
     match step
-      case InsertStep(key, value) => Insert(c, v, v', key, value)
-      case QueryStep(key, output) => Query(c, v, v', key, output)
-      case FillDefaultStep(key) => FillDefault(c, v, v', key)
+      case InsertStep(key, value) => Insert(c_, v_, v_', key, value)
+      case QueryStep(key, output) => Query(c_, v_, v_', key, output)
+      case FillDefaultStep(key) => FillDefault(c_, v_, v_', key)
   }
 
-  predicate LocalOp(c: Constants, v: Variables, v': Variables)
+  predicate LocalOp(c_: Constants, v_: Variables, v_': Variables)
   {
-    exists step :: LocalOpStep(c, v, v', step)
+    exists step :: LocalOpStep(c_, v_, v_', step)
   }
 
   datatype Message = TransferKey(k: Key, value: Value)
@@ -114,16 +114,16 @@ module Host {
   // System-partial-actions for message transmission.
   // A matched pair of these happen together atomically, so it's a
   // "synchronous" message delivery model. (We'll add more realism later.)
-  predicate Send(c: Constants, v: Variables, v': Variables, msg: Message)
+  predicate Send(c_: Constants, v_: Variables, v_': Variables, msg: Message)
   {
-    && msg.k in v.m // can only give away what Abstraction'm authoritative for
-    && v.m[msg.k] == msg.value  // transmit the correct value
-    && v'.m == map k | k in v.m && k!=msg.k :: v.m[k] // forget this key
+    && msg.k in v_.m // can only give away what I'm authoritative for
+    && v_.m[msg.k] == msg.value  // transmit the correct value
+    && v_'.m == map k | k in v_.m && k!=msg.k :: v_.m[k] // forget this key
   }
 
-  predicate Receive(c: Constants, v: Variables, v': Variables, msg: Message)
+  predicate Receive(c_: Constants, v_: Variables, v_': Variables, msg: Message)
   {
-    && v'.m == v.m[msg.k := msg.value]  // learn the new key,value pair.
+    && v_'.m == v_.m[msg.k := msg.value]  // learn the new key,value pair.
   }
 }
 
@@ -137,52 +137,52 @@ module System {
 
   datatype Variables = Variables(hosts: seq<Host.Variables>)
   {
-    predicate WF(c: Constants) { |hosts| == |c.hosts| }
+    predicate WF(c_: Constants) { |hosts| == |c_.hosts| }
   }
   
-  predicate Init(c: Constants, v: Variables)
+  predicate Init(c_: Constants, v_: Variables)
   {
-    && v.WF(c)
-    && (forall i:nat | c.ValidHost(i) :: Host.Init(c.hosts[i], v.hosts[i], i))
+    && v_.WF(c_)
+    && (forall i:nat | c_.ValidHost(i) :: Host.Init(c_.hosts[i], v_.hosts[i], i))
   }
 
-  predicate LocalOp(c: Constants, v: Variables, v': Variables, i: nat)
+  predicate LocalOp(c_: Constants, v_: Variables, v_': Variables, i: nat)
   {
-    && v.WF(c)
-    && v'.WF(c)
-    && c.ValidHost(i)
-    && Host.LocalOp(c.hosts[i], v.hosts[i], v'.hosts[i])
+    && v_.WF(c_)
+    && v_'.WF(c_)
+    && c_.ValidHost(i)
+    && Host.LocalOp(c_.hosts[i], v_.hosts[i], v_'.hosts[i])
     // all other host state UNCHANGED
-    && (forall j:nat | c.ValidHost(j) && j!=i :: v'.hosts[j] == v.hosts[j])
+    && (forall j:nat | c_.ValidHost(j) && j!=i :: v_'.hosts[j] == v_.hosts[j])
   }
 
-  predicate TransmitOp(c: Constants, v: Variables, v': Variables, src: nat, dst: nat, message: Host.Message)
+  predicate TransmitOp(c_: Constants, v_: Variables, v_': Variables, src: nat, dst: nat, message: Host.Message)
   {
-    && v.WF(c)
-    && v'.WF(c)
-    && c.ValidHost(src)
-    && c.ValidHost(dst)
-    && Host.Send(c.hosts[src], v.hosts[src], v'.hosts[src], message)
-    && Host.Receive(c.hosts[dst], v.hosts[dst], v'.hosts[dst], message)
+    && v_.WF(c_)
+    && v_'.WF(c_)
+    && c_.ValidHost(src)
+    && c_.ValidHost(dst)
+    && Host.Send(c_.hosts[src], v_.hosts[src], v_'.hosts[src], message)
+    && Host.Receive(c_.hosts[dst], v_.hosts[dst], v_'.hosts[dst], message)
     // all other host state UNCHANGED
-    && (forall j:nat | c.ValidHost(j) && j!=src && j!=dst
-        :: v'.hosts[j] == v.hosts[j])
+    && (forall j:nat | c_.ValidHost(j) && j!=src && j!=dst
+        :: v_'.hosts[j] == v_.hosts[j])
   }
 
   datatype Step =
     | LocalOpStep(i:nat)
     | TransmitOpStep(src:nat, dst:nat, message:Host.Message)
 
-  predicate NextStep(c: Constants, v: Variables, v': Variables, step:Step)
+  predicate NextStep(c_: Constants, v_: Variables, v_': Variables, step:Step)
   {
     match step
-      case LocalOpStep(i) => LocalOp(c, v, v', i)
-      case TransmitOpStep(src, dst, message) => TransmitOp(c, v, v', src, dst, message)
+      case LocalOpStep(i) => LocalOp(c_, v_, v_', i)
+      case TransmitOpStep(src, dst, message) => TransmitOp(c_, v_, v_', src, dst, message)
   }
 
-  predicate Next(c: Constants, v: Variables, v': Variables)
+  predicate Next(c_: Constants, v_: Variables, v_': Variables)
   {
-    exists step :: NextStep(c, v, v', step)
+    exists step :: NextStep(c_, v_, v_', step)
   }
 }
 
@@ -191,32 +191,32 @@ module RefinementProof {
   import MapSpec
   import opened System
 
-  predicate HostHasKey(c: Constants, v: Variables, i:nat, k:Key)
-    requires v.WF(c)
+  predicate HostHasKey(c_: Constants, v_: Variables, i:nat, k:Key)
+    requires v_.WF(c_)
   {
-    && c.ValidHost(i)
-    && k in v.hosts[i].m
+    && c_.ValidHost(i)
+    && k in v_.hosts[i].m
   }
 
   // Pulling the choose out into its own function is sometimes necessary due
   // to a (deliberate) stupidity in Dafny: it doesn't treat :| expressions
   // as subsitution-equivalent, even though the are (as evidenced by pulling
   // one into a function).
-  function TheHostWithKey(c: Constants, v: Variables, k:Key) : nat
-    requires v.WF(c)
-    requires exists i :: HostHasKey(c, v, i, k);
+  function TheHostWithKey(c_: Constants, v_: Variables, k:Key) : nat
+    requires v_.WF(c_)
+    requires exists i :: HostHasKey(c_, v_, i, k);
   {
-    var i:nat :| HostHasKey(c, v, i, k);
+    var i:nat :| HostHasKey(c_, v_, i, k);
     i
   }
 
 
-  function Ikey(c: Constants, v: Variables, key:Key) : Value
-    requires v.WF(c)
+  function Ikey(c_: Constants, v_: Variables, key:Key) : Value
+    requires v_.WF(c_)
   {
-    if exists idx :: HostHasKey(c, v, idx, key)
+    if exists idx :: HostHasKey(c_, v_, idx, key)
     then
-      v.hosts[TheHostWithKey(c, v, key)].m[key]
+      v_.hosts[TheHostWithKey(c_, v_, key)].m[key]
     else DefaultValue()
   }
 
@@ -225,134 +225,134 @@ module RefinementProof {
   // is finite for the map comprehension in Abstraction().
   // (An alternative would be to switch to imaps -- maps with potentially-infinite
   // domains -- but that would require making the spec fancier. This was a compromise.)
-  function AllKeysRecurse(c: Constants, v: Variables, count: nat) : set<Key>
-    requires v.WF(c)
-    requires count <= |c.hosts|
+  function AllKeysRecurse(c_: Constants, v_: Variables, count: nat) : set<Key>
+    requires v_.WF(c_)
+    requires count <= |c_.hosts|
   {
-    if count==0 then {} else AllKeysRecurse(c, v, count-1) + v.hosts[count-1].m.Keys
+    if count==0 then {} else AllKeysRecurse(c_, v_, count-1) + v_.hosts[count-1].m.Keys
   }
 
-  function AllKeys(c: Constants, v: Variables) : set<Key>
-    requires v.WF(c)
+  function AllKeys(c_: Constants, v_: Variables) : set<Key>
+    requires v_.WF(c_)
   {
-    AllKeysRecurse(c, v, |c.hosts|)
+    AllKeysRecurse(c_, v_, |c_.hosts|)
   }
 
-  function Abstraction(c: Constants, v: Variables) : MapSpec.Variables
-    requires v.WF(c)
+  function Abstraction(c_: Constants, v_: Variables) : MapSpec.Variables
+    requires v_.WF(c_)
   {
-    MapSpec.Variables(map k | k in AllKeys(c, v) :: Ikey(c, v, k))
+    MapSpec.Variables(map k | k in AllKeys(c_, v_) :: Ikey(c_, v_, k))
   }
 
-  predicate Inv(c: Constants, v: Variables)
+  predicate Inv(c_: Constants, v_: Variables)
   {
-    && v.WF(c)
+    && v_.WF(c_)
     // No two distinct hosts have the same key.
     && (forall k, i:nat, j:nat
-        | && c.ValidHost(i) && c.ValidHost(j)
-          && k in v.hosts[i].m && k in v.hosts[j].m
+        | && c_.ValidHost(i) && c_.ValidHost(j)
+          && k in v_.hosts[i].m && k in v_.hosts[j].m
         :: i == j
       )
   }
 
-//  lemma InitAllKeysEmpty(c: Constants, v: Variables, count: nat)
-//    requires Init(c, v)
-//    requires count <= |c.hosts|
-//    ensures AllKeysRecurse(c, v, count) == {}
+//  lemma InitAllKeysEmpty(c_: Constants, v_: Variables, count: nat)
+//    requires Init(c_, v_)
+//    requires count <= |c_.hosts|
+//    ensures AllKeysRecurse(c_, v_, count) == {}
 //  {
 //  }
 //
-  lemma AllKeysMembership(c: Constants, v: Variables, count: nat)
-    requires Inv(c, v)
-    requires count <= |c.hosts|
+  lemma AllKeysMembership(c_: Constants, v_: Variables, count: nat)
+    requires Inv(c_, v_)
+    requires count <= |c_.hosts|
     ensures forall k ::
-      (k in AllKeysRecurse(c, v, count) <==> exists i:nat :: i<count && k in v.hosts[i].m)
+      (k in AllKeysRecurse(c_, v_, count) <==> exists i:nat :: i<count && k in v_.hosts[i].m)
   {
   }
 
-  lemma InitRefines(c: Constants, v: Variables)
-    requires Init(c, v)
-    ensures MapSpec.Init(Abstraction(c, v))
-    ensures Inv(c, v)
+  lemma InitRefines(c_: Constants, v_: Variables)
+    requires Init(c_, v_)
+    ensures MapSpec.Init(Abstraction(c_, v_))
+    ensures Inv(c_, v_)
   {
-   // InitAllKeysEmpty(c, v, |c.hosts|);
-    AllKeysMembership(c, v, |c.hosts|);
+   // InitAllKeysEmpty(c_, v_, |c_.hosts|);
+    AllKeysMembership(c_, v_, |c_.hosts|);
   }
 
-  lemma InsertPreservesInvAndRefines(c: Constants, v: Variables, v': Variables, insertHost: nat, insertedKey: Key, value: Value)
-    requires Inv(c, v)
-    requires Next(c, v, v')
-    requires c.ValidHost(insertHost)
-    requires (forall j:nat | c.ValidHost(j) && j!=insertHost :: v'.hosts[j] == v.hosts[j]);
-    requires Host.Insert(c.hosts[insertHost], v.hosts[insertHost], v'.hosts[insertHost], insertedKey, value)
-    ensures Inv(c, v')
-    ensures MapSpec.Next(Abstraction(c, v), Abstraction(c, v'))
+  lemma InsertPreservesInvAndRefines(c_: Constants, v_: Variables, v_': Variables, insertHost: nat, insertedKey: Key, value: Value)
+    requires Inv(c_, v_)
+    requires Next(c_, v_, v_')
+    requires c_.ValidHost(insertHost)
+    requires (forall j:nat | c_.ValidHost(j) && j!=insertHost :: v_'.hosts[j] == v_.hosts[j]);
+    requires Host.Insert(c_.hosts[insertHost], v_.hosts[insertHost], v_'.hosts[insertHost], insertedKey, value)
+    ensures Inv(c_, v_')
+    ensures MapSpec.Next(Abstraction(c_, v_), Abstraction(c_, v_'))
   {
-    var im := Abstraction(c, v).m;
-    var im' := Abstraction(c, v').m;
+    var im := Abstraction(c_, v_).m;
+    var im' := Abstraction(c_, v_').m;
 
     forall k
       ensures k in im' <==> k in im || k == insertedKey // domain
       ensures k in im' ==> (im'[k] == if k==insertedKey then value else im[k])  // value
     {
-      AllKeysMembership(c, v', |c.hosts|);
-      // Narrowing the calls to AllKeysMembership(v) helps z3 save 15s!
-      // (But domain proof can be replaced with just AllKeysMembership(v);AllKeysMembership(v') and it'll still work.)
+      AllKeysMembership(c_, v_', |c_.hosts|);
+      // Narrowing the calls to AllKeysMembership(v_) helps z3 save 15s!
+      // (But domain proof can be replaced with just AllKeysMembership(v_);AllKeysMembership(v_') and it'll still work.)
       if k == insertedKey {
       } else if k in im' {
-        assert k in im by { AllKeysMembership(c, v, |c.hosts|); }
+        assert k in im by { AllKeysMembership(c_, v_, |c_.hosts|); }
       } else if k in im {
-        assert k in im' by { AllKeysMembership(c, v, |c.hosts|); }
+        assert k in im' by { AllKeysMembership(c_, v_, |c_.hosts|); }
       }
 
       if k in im' {
         if k==insertedKey {
-          assert HostHasKey(c, v', insertHost, k);  // trigger
-          assert Ikey(c, v', k) == value; // trigger
+          assert HostHasKey(c_, v_', insertHost, k);  // trigger
+          assert Ikey(c_, v_', k) == value; // trigger
         } else {
-          var ihost:nat :| ihost<|c.hosts| && k in v'.hosts[ihost].m;
-          assert forall j | c.ValidHost(j) && j!=ihost :: !HostHasKey(c, v, j, k);  // trigger
-          assert HostHasKey(c, v', ihost, k) by { AllKeysMembership(c, v, |c.hosts|); }
-          assert TheHostWithKey(c, v', k) == ihost; // witness
+          var ihost:nat :| ihost<|c_.hosts| && k in v_'.hosts[ihost].m;
+          assert forall j | c_.ValidHost(j) && j!=ihost :: !HostHasKey(c_, v_, j, k);  // trigger
+          assert HostHasKey(c_, v_', ihost, k) by { AllKeysMembership(c_, v_, |c_.hosts|); }
+          assert TheHostWithKey(c_, v_', k) == ihost; // witness
           assert im'[k] == im[k]; // trigger
         }
       }
     }
 
-    assert MapSpec.InsertOp(Abstraction(c, v), Abstraction(c, v'), insertedKey, value); // bizarre magic backwards causality-violating trigger
-    assert MapSpec.NextStep(Abstraction(c, v), Abstraction(c, v'), MapSpec.InsertOpStep(insertedKey, value)); // witness
+    assert MapSpec.InsertOp(Abstraction(c_, v_), Abstraction(c_, v_'), insertedKey, value); // bizarre magic backwards causality-violating trigger
+    assert MapSpec.NextStep(Abstraction(c_, v_), Abstraction(c_, v_'), MapSpec.InsertOpStep(insertedKey, value)); // witness
   }
 
-  lemma NextPreservesInvAndRefines(c: Constants, v: Variables, v': Variables)
-    requires Inv(c, v)
-    requires Next(c, v, v')
-    ensures Inv(c, v')
-    ensures MapSpec.Next(Abstraction(c, v), Abstraction(c, v'))
+  lemma NextPreservesInvAndRefines(c_: Constants, v_: Variables, v_': Variables)
+    requires Inv(c_, v_)
+    requires Next(c_, v_, v_')
+    ensures Inv(c_, v_')
+    ensures MapSpec.Next(Abstraction(c_, v_), Abstraction(c_, v_'))
   {
-    var step :| NextStep(c, v, v', step);
+    var step :| NextStep(c_, v_, v_', step);
     match step
       case LocalOpStep(idx) => {
-        var hstep :| Host.LocalOpStep(c.hosts[idx], v.hosts[idx], v'.hosts[idx], hstep);
+        var hstep :| Host.LocalOpStep(c_.hosts[idx], v_.hosts[idx], v_'.hosts[idx], hstep);
         match hstep
-          case InsertStep(k, value) => InsertPreservesInvAndRefines(c, v, v', idx, k, value);
+          case InsertStep(k, value) => InsertPreservesInvAndRefines(c_, v_, v_', idx, k, value);
           case QueryStep(k, output) => {
             assume false;
-            assert Inv(c, v');
-            assert Abstraction(c, v) == Abstraction(c, v');
-            assert MapSpec.Next(Abstraction(c, v), Abstraction(c, v'));
+            assert Inv(c_, v_');
+            assert Abstraction(c_, v_) == Abstraction(c_, v_');
+            assert MapSpec.Next(Abstraction(c_, v_), Abstraction(c_, v_'));
           }
           case FillDefaultStep(k) => {
             assume false;
-            assert Inv(c, v');
-            assert Abstraction(c, v) == Abstraction(c, v');
-            assert MapSpec.Next(Abstraction(c, v), Abstraction(c, v'));
+            assert Inv(c_, v_');
+            assert Abstraction(c_, v_) == Abstraction(c_, v_');
+            assert MapSpec.Next(Abstraction(c_, v_), Abstraction(c_, v_'));
           }
       }
       case TransmitOpStep(src, dst, message) => {
         assume false;
-        assert Inv(c, v');
-        assert Abstraction(c, v) == Abstraction(c, v');
-        assert MapSpec.Next(Abstraction(c, v), Abstraction(c, v'));
+        assert Inv(c_, v_');
+        assert Abstraction(c_, v_) == Abstraction(c_, v_');
+        assert MapSpec.Next(Abstraction(c_, v_), Abstraction(c_, v_'));
       }
   }
 }
